theories/L6_PCPS/dead_param_elim_correct.v
@@ -1,0 +1,362 @@
+Require Import L6.cps L6.identifiers L6.ctx L6.set_util L6.state
+        L6.dead_param_elim L6.Ensembles_util L6.tactics L6.map_util
+        L6.hoisting.
+Require Import compcert.lib.Coqlib Common.compM Common.Pipeline_utils.
+Require Import Coq.Lists.List Coq.MSets.MSets Coq.MSets.MSetRBT Coq.Numbers.BinNums
+        Coq.NArith.BinNat Coq.PArith.BinPos Coq.Sets.Ensembles Omega
+        maps_util.
+Require Import ExtLib.Structures.Monads ExtLib.Data.Monads.StateMonad.
+Import ListNotations Nnat.
+
+
+Import MonadNotation.
+Open Scope monad_scope.
+
+Open Scope ctx_scope.
+Open Scope fun_scope.
+Close Scope Z_scope.
+
+
+Inductive Dead_in_args (S : Ensemble var) : list var -> list bool -> Prop :=
+| Live_nil : Dead_in_args S [] []
+| ALive_cons_Dead :
+    forall (x : var) (xs : list var) (bs: list bool),
+      Dead_in_args S xs bs ->
+      Dead_in_args S (x :: xs) (false :: bs)
+| ALive_cons_Live :
+    forall (x : var) (xs : list var) (bs: list bool),
+      Dead_in_args S xs bs ->
+      ~ x \in S -> 
+      Dead_in_args S (x :: xs) (true :: bs).
+
+
+Fixpoint dead_args (ys : list var) (bs : list bool) : list var := 
+  match ys, bs with 
+  | [], [] => ys
+  | y :: ys', b :: bs' => 
+    if b then (dead_args ys' bs')
+    else y :: dead_args ys' bs'
+| _, _ => ys
+end. 
+
+Inductive Dead (S : Ensemble var) (L : live_fun) : exp -> Prop :=
+| Live_Constr : 
+    forall (x : var) (ys : list var) (ct : ctor_tag) (e : exp), 
+      Disjoint _ (FromList ys) S -> 
+      Dead S L e ->
+      Dead S L (Econstr x ct ys e)
+| Live_Prim : 
+  forall (x : var) (g : prim) (ys : list var) (e : exp), 
+    Disjoint _ (FromList ys) S -> 
+    Dead S L e ->
+    Dead S L (Eprim x g ys e)
+| Live_Proj : 
+    forall (x : var) (ct : ctor_tag) (n : N) (y : var) (e : exp), 
+      ~ y \in S ->
+     Dead S L e ->
+     Dead S L (Eproj x ct n y e)
+| Live_Case: 
+    forall (x : var) (ce : list (ctor_tag * exp)),
+      ~ x \in S ->
+      Forall (fun p => Dead S L (snd p)) ce -> 
+      Dead S L (Ecase x ce)
+| Live_Halt : 
+    forall (x : var),
+      ~ x \in S ->
+      Dead S L (Ehalt x)
+| Live_App_Unknown :
+    forall (f : var) (ys : list var) (ft : fun_tag),
+      ~ f \in S ->
+      Disjoint _ (FromList ys) S -> 
+      L ! f = None -> 
+      Dead S L (Eapp f ft ys)
+| Live_App_Known :
+    forall (f : var) (ys : list var) (ft : fun_tag) (bs : list bool),
+      L ! f = Some bs ->
+      ~ f \in S ->
+      Disjoint _ S (FromList (live_args ys bs)) ->
+      Dead S L (Eapp f ft ys)
+| Live_LetApp_Unknown :
+    forall (x f : var) (ys : list var) (ft : fun_tag) (e : exp),
+      ~ f \in S ->
+      Disjoint _ (FromList ys) S -> 
+      L ! f = None -> 
+      Dead S L (Eletapp x f ft ys e)
+| Live_LetApp_Known :
+    forall (x f : var) (ys : list var) (ft : fun_tag) (e : exp) (bs : list bool),
+      L ! f = Some bs ->
+      ~ f \in S ->
+      Disjoint _ S (FromList (live_args ys bs)) ->      
+      Dead S L (Eletapp x f ft ys e). 
+  
+  
+Definition live_map_sound (B : fundefs) (L : live_fun) :=
+  forall f ft xs e bs,
+    fun_in_fundefs B (f, ft, xs, e) ->
+    L ! f = Some bs -> 
+    Dead (FromList (dead_args xs bs)) L e. 
+
+Definition live_fun_args (L : live_fun) (f : var) (xs : list var) :=
+  exists bs, L ! f = Some bs /\ length xs = length bs. 
+
+Definition live_fun_fundefs (L : live_fun) (B : fundefs) :=
+  forall f ft xs e,
+    fun_in_fundefs B (f, ft, xs, e) ->
+    live_fun_args L f xs.
+
+(* Lemmas about [live] *)
+
+Lemma live_diff B L L' d :
+  live B L d = Some (L', false) ->
+  d = false.
+Proof.
+  revert L L' d. induction B; simpl; intros L L' d Hl; eauto.
+  - destruct (update_live_fun L v l (live_expr L e PS.empty)) as [ [L'' d''] | ].
+    + eapply IHB in Hl. destruct d; eauto. destruct d''; eauto.
+    + inv Hl.
+  - inv Hl; eauto.
+Qed.
+
+Lemma update_live_fun_false L L' f xs S :
+  live_fun_args L f xs ->
+  update_live_fun L f xs S = Some (L', false) ->
+  exists bs,
+    get_fun_vars L f = Some bs /\
+    L = L' /\ Disjoint _ (FromSet S) (FromList (dead_args xs bs)).
+Proof.
+  intros Hlive Hl.
+  unfold update_live_fun in Hl.
+  destruct (get_fun_vars L f) eqn:Hf; try congruence.
+  eexists.
+  split. reflexivity. 
+  destruct Hlive. destructAll.
+  unfold get_fun_vars in *. subst_exp.
+  destruct ((fix update_bs (xs : list PS.elt) (bs : list bool) {struct xs} :
+               list bool * bool :=
+               match xs with
+               | [] => ([], false)
+               | x :: xs0 =>
+                 match bs with
+                 | [] => ([], false)
+                 | b :: bs0 =>
+                   let (bs', d) := update_bs xs0 bs0 in
+                   (PS.mem x S || b :: bs', negb (eqb b (PS.mem x S)) || d)
+                 end
+               end) xs l) as [bs diff] eqn:Hupd.
+  inv Hl.
+  destruct diff. congruence. inv H2.
+  assert (Hsuff : bs = l /\ Disjoint positive (FromSet S) (FromList (dead_args xs l))).
+  { clear H. revert l bs Hupd H0.
+    induction xs; intros l bs Hupd Heq.
+    - inv Hupd.
+      destruct l; inv Heq; eauto.
+      split; eauto. simpl. normalize_sets. sets.
+    - destruct l. now inv Heq. 
+      simpl in *.
+      destruct ((fix update_bs (xs : list PS.elt) (bs : list bool) {struct xs} :
+                   list bool * bool :=
+                   match xs with
+                   | [] => ([], false)
+                   | x :: xs0 =>
+                     match bs with
+                   | [] => ([], false)
+                   | b :: bs0 =>
+                     let (bs', d) := update_bs xs0 bs0 in
+                     (PS.mem x S || b :: bs',
+                      negb (eqb b (PS.mem x S)) || d)
+                     end
+                   end) xs l) as [bs' diff] eqn:Hrec.
+      inv Hupd.
+      eapply orb_false_iff in H1. inv H1. 
+      eapply negb_false_iff in H. 
+      eapply (eqb_true_iff b) in H. subst.
+      inv Heq. specialize (IHxs l bs' Hrec H0). 
+      destructAll.
+      rewrite orb_diag. split. reflexivity.
+      
+      destruct (PS.mem a S) eqn:Hmem. eassumption.
+      normalize_sets. eapply Union_Disjoint_r; [| eassumption ].  
+      eapply Disjoint_Singleton_r. 
+      intros Hc. eapply FromSet_sound in Hc; [| reflexivity ].
+      eapply PS.mem_spec in Hc. congruence. }
+  split. reflexivity.
+  inv Hsuff. eassumption.
+Qed.
+
+
+(* Lemma live_expr_monotonic L e Q1 Q2 : *)
+(*   FromSet Q1 \subset FromSet Q2 -> *)
+(*   FromSet (live_expr L e Q1) \subset FromSet (live_expr L e Q2). *)
+(* Proof. *)
+(*   revert Q1 Q2. induction e using exp_ind'; intros Q1 Q2 Hsub; simpl; eauto. *)
+(*   - eapply IHe. rewrite !FromSet_union_list; sets. *)
+(*   - rewrite !FromSet_add; sets. *)
+(*   - eapply IHe. rewrite !FromSet_add. sets. *)
+(*   - eapply IHe.  *)
+
+(*     simpl in *.  *)
+
+(*     ~eapply IHe. rewrite !FromSet_union_list; sets. *)
+(*   - *)
+(*     try now (eapply Included_trans; [| eapply IHe ]; rewrite FromSet_union_list; sets). *)
+(*   - rewrite FromSet_add; sets. *)
+(*   - simpl in *. eapply Included_trans. eapply IHe0. *)
+(*     assert (Hsub : FromSet (PS.add v Q) \subset FromSet (live_expr L e (PS.add v Q))). *)
+(*     { eapply IHe. } *)
+(*     clear IHe. revert Hsub. generalize (PS.add v Q), (live_expr L e (PS.add v Q)). *)
+(*     clear IHe0. induction l; intros. *)
+(*     + eassumption. *)
+(*     + destruct a. eapply IHl; eauto. *)
+(*       2:{ reflexivity. } *)
+
+Lemma add_fun_vars_subset L v l Q : 
+  FromSet Q \subset FromSet (add_fun_vars L v l Q).
+Proof.
+  unfold add_fun_vars. 
+  destruct (get_fun_vars L v); rewrite FromSet_union_list; sets.
+Qed.
+        
+  
+Lemma live_expr_subset L e Q :
+  FromSet Q \subset FromSet (live_expr L e Q).
+Proof.
+  revert Q; induction e using exp_ind'; intros Q; simpl;
+    try now (eapply Included_trans; [| eapply IHe ]; rewrite FromSet_union_list; sets).
+  - rewrite FromSet_add; sets.
+  - simpl in *. rewrite !FromSet_add. setoid_rewrite FromSet_add in IHe0.
+    eapply Included_trans; [| eapply IHe0 ].
+    eapply IHe.
+  - eapply Included_trans; [| eapply IHe ].
+    rewrite FromSet_add; sets.
+  - eapply Included_trans; [| eapply IHe ].
+    eapply Included_trans; [| eapply add_fun_vars_subset ].
+    rewrite !FromSet_add; sets.
+  - sets. 
+  - eapply Included_trans; [| eapply add_fun_vars_subset ].
+    rewrite FromSet_add; sets.
+  - rewrite FromSet_add; sets.  
+Qed.
+
+Lemma fold_left_live_expr_subset L S (P : list (ctor_tag * exp)) :
+  FromSet S \subset FromSet (fold_left (fun (S : PS.t) '(_, e') => live_expr L e' S) P S).
+Proof.
+  revert S. induction P; simpl; intros; sets.
+  destruct a. eapply Included_trans; [| eapply IHP ].
+  eapply live_expr_subset.
+Qed.
+  
+Lemma live_args_subset ys bs:
+  FromList (live_args ys bs) \subset FromList ys.
+Proof.
+  revert bs; induction ys; intros [ | [|] bs ]; simpl; sets.
+  - repeat normalize_sets. sets.
+  - repeat normalize_sets. sets.
+Qed.  
+
+
+Lemma live_expr_sound Q L e S :
+  no_fun e ->
+  Disjoint _ (FromSet (live_expr L e Q)) S ->
+  Dead S L e.
+Proof.
+  revert Q; induction e using exp_ind'; intros Q; simpl; intros Hnf Hdis; inv Hnf.  
+  - econstructor.
+    + repeat normalize_bound_var_in_ctx. repeat normalize_occurs_free_in_ctx.
+      eapply Disjoint_Included_l; [| eassumption ].
+      eapply Included_trans; [| eapply live_expr_subset ].
+      rewrite FromSet_union_list. sets.
+    + eapply IHe; eauto.
+  - rewrite FromSet_add in *.
+    econstructor; eauto. intros Hc.
+    eapply Hdis. econstructor; eauto.
+  - rewrite FromSet_add in *. econstructor.
+    + intros Hc. eapply Hdis. econstructor; eauto.
+    + econstructor. eapply IHe; eauto.
+      * eapply Disjoint_Included_l; [| eassumption ].
+        eapply Included_Union_preserv_r.
+        eapply fold_left_live_expr_subset.
+      * assert (Hsuff : Dead S L (Ecase v l)).
+        { eapply IHe0; eauto.
+          eapply Disjoint_Included_l; [| eassumption ].
+          simpl. rewrite FromSet_add. sets. }
+        inv Hsuff. eassumption.
+  - econstructor.
+    + repeat normalize_bound_var_in_ctx. repeat normalize_occurs_free_in_ctx.
+      intros Hc. 
+      eapply Hdis; eauto. econstructor; eauto. eapply live_expr_subset.
+      rewrite FromSet_add. sets.
+    + eapply IHe; eauto.
+  - destruct (L ! f) eqn:Heq.
+    + eapply Live_LetApp_Known. eassumption. 
+      * intros Hc. eapply Hdis. constructor; eauto.
+        eapply live_expr_subset.
+        eapply add_fun_vars_subset. rewrite FromSet_add. sets.
+      * repeat normalize_bound_var_in_ctx. repeat normalize_occurs_free_in_ctx.
+        eapply Disjoint_sym. eapply Disjoint_Included_l; [| eassumption ].
+        eapply Included_trans; [| eapply live_expr_subset ].
+        unfold add_fun_vars, get_fun_vars. rewrite Heq.
+        rewrite FromSet_union_list.  sets.
+    + eapply Live_LetApp_Unknown; eauto.
+      * intros Hc. eapply Hdis. constructor; eauto.
+        eapply live_expr_subset.
+        eapply add_fun_vars_subset. rewrite FromSet_add. sets.
+      * repeat normalize_bound_var_in_ctx. repeat normalize_occurs_free_in_ctx.
+        eapply Disjoint_Included_l; [| eassumption ].
+        eapply Included_trans; [| eapply live_expr_subset ].
+        unfold add_fun_vars. unfold get_fun_vars. rewrite Heq.
+        rewrite FromSet_union_list. sets.
+  - destruct (L ! v) eqn:Heq.
+    + eapply Live_App_Known. eassumption. 
+      * intros Hc. eapply Hdis. constructor; eauto.
+        eapply add_fun_vars_subset. rewrite FromSet_add. sets.
+      * repeat normalize_bound_var_in_ctx. repeat normalize_occurs_free_in_ctx.
+        eapply Disjoint_sym. eapply Disjoint_Included_l; [| eassumption ].
+        unfold add_fun_vars, get_fun_vars. rewrite Heq.
+        rewrite FromSet_union_list.  sets.
+    + eapply Live_App_Unknown; eauto.
+      * intros Hc. eapply Hdis. constructor; eauto.
+        eapply add_fun_vars_subset. rewrite FromSet_add. sets.
+      * repeat normalize_bound_var_in_ctx. repeat normalize_occurs_free_in_ctx.
+        eapply Disjoint_Included_l; [| eassumption ].
+        unfold add_fun_vars. unfold get_fun_vars. rewrite Heq.
+        rewrite FromSet_union_list. sets.
+  - econstructor.
+    + repeat normalize_bound_var_in_ctx. repeat normalize_occurs_free_in_ctx.
+      eapply Disjoint_Included_l; [| eassumption ].
+      eapply Included_trans; [| eapply live_expr_subset ].
+      rewrite FromSet_union_list. sets.
+    + eapply IHe; eauto.
+  - econstructor.
+    + repeat normalize_bound_var_in_ctx. repeat normalize_occurs_free_in_ctx.
+      intros Hc. eapply Hdis. constructor; eauto.
+      rewrite FromSet_add. now sets. 
+Qed. 
+      
+Lemma live_correct L L' B :
+  no_fun_defs B -> (* no nested functions in B *)
+  live_fun_fundefs L B -> (* arity in map is consistent *)
+  live B L false = Some (L', false) -> 
+  L = L' /\ live_map_sound B L.
+Proof.
+  revert L L'; induction B; simpl; intros L L' Hnf Hlive Hl.
+  - destruct (update_live_fun L v l (live_expr L e PS.empty)) as [[L'' b] | ] eqn:Heq.
+    2:{ congruence. }
+    
+    assert (Hd := live_diff _ _ _ _ Hl). destruct b; inv Hd.
+    simpl in *. 
+    edestruct update_live_fun_false; try eassumption.
+    eapply Hlive.  now left. 
+    destructAll.
+    eapply IHB in Hl. inv Hl.
+    split. reflexivity.
+    { intro; intros.  inv H0.
+      - inv H4. eapply live_expr_sound. inv Hnf. eassumption.
+        unfold get_fun_vars in *. subst_exp.
+        eassumption. 
+      - eapply H2. eassumption. eassumption. } 
+    inv Hnf. eassumption.
+    intro; intros. 
+    eapply Hlive. now right; eauto. 
+  - inv Hl. split; eauto.
+    intro; intros. inv H.
+Qed. 
